further cleanup

ironfleet/src/Dafny/Distributed/Services/WS/WS.s.dfy
@@ -5,34 +5,50 @@ module WS__WS_s {
 import opened Native__Io_s
 
 type HTTPRequest = seq<char>
-type HTTPResponse = seq<byte>
+type HTTPResponse = seq<char>
 
 predicate SpecInit()
 {
     true
 }
 
+function GetProtocolVersion() : string
+{
+    "HTTP/1.1"
+}
+
+function GetHTTPCode(responseCase:string) : string
+{
+    if responseCase == "OK" then "200"
+    else if responseCase == "Not Found" then "400"
+    else "404"
+}
+
+function LineBreaks() : string
+{
+    "\n\r\n\r"
+}
+
 // supports only a very primitive request format at the moment
 predicate IsValidHTTPReq(req:HTTPRequest)
 {
-    exists op,filePath,ver :: (req == op + " " + filePath + " " + ver) 
-                               && op == "GET" && |filePath| > 1 
-                               && ver == "HTTP/1.0" 
+    exists filePath :: |filePath| > 1 && (req == "GET " + filePath + " " + GetProtocolVersion())
 }
 
-// TODO: HTTP response should include headers
+function BytesToString(b:seq<byte>) : seq<char>
+
+function StringToBytes(arr:seq<char>) : seq<byte>
+
+// TODO: need to set other headers
 predicate Get(fs:FileSystemState, req:HTTPRequest, res:HTTPResponse)
     requires fs != null;
 {
-       // Is there a way to avoid duplicating this?
        fs != null
     && if IsValidHTTPReq(req) then
-        (exists op,filePath,ver :: (req == op + " " + filePath + " " + ver) 
-                               && op == "GET" && |filePath| > 1 
-                               && ver == "HTTP/1.0" 
-                               && (res == if fs.file_exists(filePath) then fs.contents(filePath[1..]) else []))
+        (exists filePath :: |filePath| > 1 
+                         && (req == "GET " + filePath + " " + GetProtocolVersion()) 
+                         && (res == if fs.file_exists(filePath[1..]) then (GetProtocolVersion() + " " + GetHTTPCode("OK") + LineBreaks() + BytesToString(fs.contents(filePath[1..]))) else GetProtocolVersion() + " " + GetHTTPCode("Not Found")))
        else
-        res == []
-         
+        res == GetProtocolVersion() + " " + GetHTTPCode("Invalid")
 }
 }
